OwlLean/TypeChecker/OwlTypecheck.lean
@@ -1,0 +1,52 @@
+import OwlLean.TypeChecker.OwlParser
+import OwlLean.TypeChecker.OwlTyping
+
+import Lean
+import Std.Data.HashMap
+open Lean Elab Meta
+
+syntax "tc" : tactic
+
+macro_rules
+  | `(tactic| tc) =>
+  `(tactic|
+    first
+    | apply has_type.T_Var
+    | apply has_type.T_IUnit
+    | apply has_type.T_Const
+    | (apply has_type.T_Op; tc; tc)
+    | (apply has_type.T_Zero; tc)
+  )
+
+def tm1 :=
+  Owl {
+    *
+  }
+
+def ty1 :=
+  OwlTy {
+    Unit
+  }
+
+-- example : True has type bool
+theorem tc1 : has_type (@empty_phi 0) empty_delta empty_gamma tm1 ty1 := by
+  tc
+
+-- test operator
+def coin_flip : Owl.op :=
+  fun (_ _ : Owl.binary) =>
+    Owl.Dist.ret (Owl.binary.bend)
+
+def tm2 :=
+  Owl {
+    ⟨coin_flip⟩ (["1101"], ["1001"])
+  }
+
+noncomputable def ty2 :=
+  OwlTy {
+    (Data ⟨Owl.L.bot⟩)
+  }
+
+-- example : True has type bool
+theorem tc2 : has_type (@empty_phi 0) empty_delta empty_gamma tm2 ty2 := by
+  tc
