OwlLean/TypeChecker/OwlTyping.lean
@@ -1,4 +1,5 @@
 import OwlLean.OwlLang.Owl
+
 open Owl
 
 -- sanity checks
